Get rid of "raw" bind

src/Distributions/UniformPowerOfTwo/Model.dfy
@@ -32,14 +32,13 @@ module UniformPowerOfTwo.Model {
   }
 
   // A tail recursive version of Sample, closer to the imperative implementation
-  function SampleTailRecursive(n: nat, u: nat := 0): Monad.RawHurd<nat>
+  function SampleTailRecursive(n: nat, u: nat := 0): Monad.Hurd<nat>
     requires n >= 1
   {
-    (s: Rand.Bitstream) =>
-      if n == 1 then
-        Monad.Result(u, s)
-      else
-        SampleTailRecursive(n / 2, if Rand.Head(s) then 2*u + 1 else 2*u)(Rand.Tail(s))
+    if n == 1 then
+      Monad.Return(u)
+    else
+      Monad.Bind(Monad.Coin, c => SampleTailRecursive(n / 2, if c then 2*u + 1 else 2*u))
   }
 
   // Equivalence of Sample and its tail-recursive version
@@ -57,7 +56,7 @@ module UniformPowerOfTwo.Model {
         SampleTailRecursive(n)(s);
         { SampleTailRecursiveEqualIfSameLog2Floor(n, Helper.Power(2, k), k, 0, s); }
         SampleTailRecursive(Helper.Power(2, k))(s);
-        Monad.RawBind(Sample(Helper.Power(2, 0)), (u: nat) => SampleTailRecursive(Helper.Power(2, k), u))(s);
+        Monad.Bind(Sample(Helper.Power(2, 0)), (u: nat) => SampleTailRecursive(Helper.Power(2, k), u))(s);
         { RelateWithTailRecursive(k, 0, s); }
         Sample(Helper.Power(2, k))(s);
         { SampleEqualIfSameLog2Floor(n, Helper.Power(2, k), k, s); }
@@ -117,11 +116,11 @@ module UniformPowerOfTwo.Model {
   // The induction invariant for the equivalence proof (generalized version of SampleCorrespondence)
   lemma RelateWithTailRecursive(l: nat, m: nat, s: Rand.Bitstream)
     decreases l
-    ensures Monad.RawBind(Sample(Helper.Power(2, m)), (u: nat) => SampleTailRecursive(Helper.Power(2, l), u))(s) == Sample(Helper.Power(2, m + l))(s)
+    ensures Monad.Bind(Sample(Helper.Power(2, m)), (u: nat) => SampleTailRecursive(Helper.Power(2, l), u))(s) == Sample(Helper.Power(2, m + l))(s)
   {
     if l == 0 {
       calc {
-        Monad.RawBind(Sample(Helper.Power(2, m)), (u: nat) => SampleTailRecursive(Helper.Power(2, l), u))(s);
+        Monad.Bind(Sample(Helper.Power(2, m)), (u: nat) => SampleTailRecursive(Helper.Power(2, l), u))(s);
         (var Result(u, s') := Sample(Helper.Power(2, m))(s); SampleTailRecursive(1, u)(s'));
         Sample(Helper.Power(2, m + l))(s);
       }
@@ -130,7 +129,7 @@ module UniformPowerOfTwo.Model {
       assert MGreaterZero: Helper.Power(2, m) >= 1 by { Helper.PowerGreater0(2, m); }
       assert L1GreaterZero: Helper.Power(2, l - 1) >= 1 by { Helper.PowerGreater0(2, l - 1); }
       calc {
-        Monad.RawBind(Sample(Helper.Power(2, m)), (u: nat) => SampleTailRecursive(Helper.Power(2, l), u))(s);
+        Monad.Bind(Sample(Helper.Power(2, m)), (u: nat) => SampleTailRecursive(Helper.Power(2, l), u))(s);
         (var Result(u, s') := Sample(Helper.Power(2, m))(s); SampleTailRecursive(Helper.Power(2, l), u)(s'));
         { reveal LGreaterZero; }
         (var Result(u, s') := Sample(Helper.Power(2, m))(s);
@@ -141,7 +140,7 @@ module UniformPowerOfTwo.Model {
         { assert Helper.Power(2, m + 1) / 2 == Helper.Power(2, m); reveal Sample(); }
         (var Result(u', s') := Sample(Helper.Power(2, m + 1))(s);
          SampleTailRecursive(Helper.Power(2, l - 1), u')(s'));
-        Monad.RawBind(Sample(Helper.Power(2, m + 1)), (u: nat) => SampleTailRecursive(Helper.Power(2, l - 1), u))(s);
+        Monad.Bind(Sample(Helper.Power(2, m + 1)), (u: nat) => SampleTailRecursive(Helper.Power(2, l - 1), u))(s);
         { RelateWithTailRecursive(l - 1, m + 1, s); }
         Sample(Helper.Power(2, m + l))(s);
       }
